a bit of progress trying to prove event_ignores_policy
shatter makes it annoying - the number of register parts produced when a
robot is destroyed will be different after putting in new policies.

perhaps we should, rather than setting arbitrary policies, require
policies of the right length. i.e., fill should always put in a
same-length arbitrary policy (when an arbitrary one is needed) rather
than what it currently does (just use an empty list).

botworld_propsScript.sml
@@ -14,6 +14,10 @@ val policy_fun_def = Define`
 fun Abbrev_intro th =
   EQ_MP (SYM(SPEC(concl th)markerTheory.Abbrev_def)) th
 
+val set_policy_def = Define`
+  set_policy r i ps =
+    r with memory updated_by (λm. if i < LENGTH ps then EL i ps else m)`;
+
 val set_policies_def = Define`
   (set_policies [] _ = []) ∧
   (set_policies rs [] = rs) ∧
@@ -28,12 +32,25 @@ val LENGTH_set_policies = Q.store_thm("LENGTH_set_policies[simp]",
 val EL_set_policies = Q.store_thm("EL_set_policies",
   `i < LENGTH rs ⇒
      EL i (set_policies rs ps) =
-     (EL i rs with memory := if i < LENGTH ps then EL i ps else (EL i rs).memory)`,
+     set_policy (EL i rs) i ps`,
   map_every qid_spec_tac[`i`,`ps`] >>
   Induct_on`rs` >> simp[] >>
   Cases_on`ps`>>simp[set_policies_def] >- (
-    rw[robot_component_equality] ) >>
-  gen_tac >> Cases >> simp[])
+    rw[robot_component_equality,set_policy_def] ) >>
+  gen_tac >> Cases >> simp[set_policy_def] >>
+  simp[robot_component_equality])
+
+val set_policies_thm = Q.store_thm("set_policies_thm",
+  `set_policies rs ps = GENLIST (λi. set_policy (EL i rs) i ps) (LENGTH rs)`,
+  rw[LIST_EQ_REWRITE,EL_set_policies]);
+
+(*
+val set_policies_append = Q.store_thm("set_policies_append",
+  `set_policies (a ++ b) ps =
+   set_policies a ps ++
+   GENLIST (λi. set_policy (EL (LENGTH a + i) b) (LENGTH a + i) ps) (LENGTH b)`,
+  rw[set_policies_thm, GENLIST_APPEND] >>
+*)
 
 val square_set_policies_def = Define`
   square_set_policies sq ps = sq with <| robots := set_policies sq.robots ps |>`;
@@ -68,46 +85,99 @@ val MAP_robot_command_set_policies = Q.store_thm("MAP_robot_command_set_policies
 val inspectShielded_ignores_policy = Q.store_thm("inspectShielded_ignores_policy[simp]",
   `n < LENGTH ls ⇒
     (inspectShielded (set_policies ls ps) n ⇔ inspectShielded ls n)`,
-  simp[inspectShielded_def] >> simp[EL_set_policies]);
+  simp[inspectShielded_def] >> simp[EL_set_policies,set_policy_def]);
 
 val destroyShielded_ignores_policy = Q.store_thm("destroyShielded_ignores_policy[simp]",
   `n < LENGTH ls ⇒
     (destroyShielded (set_policies ls ps) n ⇔ destroyShielded ls n)`,
-  simp[destroyShielded_def] >> simp[EL_set_policies]);
+  simp[destroyShielded_def] >> simp[EL_set_policies,set_policy_def]);
 
 val fix_inspected_def = Define`
-  (fix_inspected ps (Inspected j r) =
-     Inspected j (r with memory := if j < LENGTH ps then EL j ps else r.memory)) ∧
+  (fix_inspected ps (Inspected j r) = Inspected j (set_policy r j ps)) ∧
   (fix_inspected _ a = a)`;
 
 val act_ignores_policy = Q.store_thm("act_ignores_policy[simp]",
   `act (square_set_policies sq ps) nb i = fix_inspected ps (act sq nb i)`,
   rw[act_def,square_set_policies_def,fix_inspected_def] >>
   rfs[EL_set_policies] >> fs[] >>
-  `r'.command = r.command` by simp[Abbr`r`] >>
+  `r'.command = r.command` by simp[Abbr`r`]
+  >- simp[set_policy_def] >>
   simp[] >>
   BasicProvers.CASE_TAC >> fs[LET_THM] >>
-  TRY (rw[fix_inspected_def]>>NO_TAC)
+  TRY (rw[fix_inspected_def]>>fs[set_policy_def]>>NO_TAC)
   >- (
     simp[Abbr`r`,canLift_def] >>
-    rw[fix_inspected_def])
+    rw[fix_inspected_def] >> fs[set_policy_def])
   >- (
-    rw[Abbr`r`,fix_inspected_def] )
+    rw[Abbr`r`,fix_inspected_def] >> fs[set_policy_def])
   >- (
     simp[o_DEF,GSYM square_set_policies_def] >>
     rw[fix_inspected_def] >>
     BasicProvers.CASE_TAC >> rw[fix_inspected_def]))
 
-(*
-val localActions_ignores_policy = Q.store_thm("localActions_ignores_policy",
-  `localActions (square_set_policies sq ps) nb = localActions sq nb`,
-  rw[localActions_def]
+val localActions_ignores_policy = Q.store_thm("localActions_ignores_policy[simp]",
+  `localActions (square_set_policies sq ps) nb = MAP (fix_inspected ps) (localActions sq nb)`,
+  rw[localActions_def,MAP_GENLIST] >>
+  AP_THM_TAC >> AP_TERM_TAC >> simp[FUN_EQ_THM])
 
+val updateInventory_ignores_policy = Q.store_thm("updateInventory_ignores_policy",
+  `i < LENGTH sq.robots ⇒
+   (updateInventory (square_set_policies sq ps) i a =
+    set_policy (updateInventory sq i a) i ps)`,
+  rw[updateInventory_def,square_set_policies_def] >>
+  rfs[EL_set_policies] >>
+  simp[Abbr`r`] >>
+  BasicProvers.CASE_TAC >> simp[set_policy_def]);
+
+val GENLIST_updateInventory_ignores_policy = Q.store_thm("GENLIST_updateInventory_ignores_policy[simp]",
+  `GENLIST (λi. updateInventory (square_set_policies sq ps) i (f i)) (LENGTH sq.robots) =
+   GENLIST (λi. set_policy (updateInventory sq i (f i)) i ps) (LENGTH sq.robots)`,
+  rw[LIST_EQ_REWRITE,updateInventory_ignores_policy])
+
+(*
 val event_ignores_policy = Q.store_thm("event_ignores_policy",
   `event (square_set_policies sq ps) nb =
    event sq nb with robotActions updated_by
-     (λls. ZIP (set_policies (MAP FST ls) ps, MAP SND ls))`,
-  rw[event_def]
+     (λls. ZIP (set_policies (MAP FST ls) ps, MAP (fix_inspected ps) (MAP SND ls)))`,
+  rw[event_def,event_component_equality] >> rw[] >>
+  `LENGTH actions = LENGTH actions' ∧
+   LENGTH veterans = LENGTH veterans' ∧
+   children = children' ∧
+   LENGTH fallen = LENGTH fallen'` by (
+     unabbrev_all_tac >> simp[] >>
+     simp[LENGTH_FLAT,MAP_GENLIST,MAP_MAP_o] >>
+     rw[] >> AP_TERM_TAC >>
+     simp[LIST_EQ_REWRITE,EL_MAP] >>
+     rw[] >- (
+       match_mp_tac EQ_SYM >>
+       BasicProvers.CASE_TAC >>
+       simp[fix_inspected_def] ) >>
+     >- (
+       match_mp_tac EQ_SYM >>
+       BasicProvers.CASE_TAC >>
+       simp[fix_inspected_def] ) >>
+     fs[MEM_MAP] >- (
+       Cases_on`y`>>fs[fix_inspected_def]>>
+       rw[] >> fs[] ) >>
+     first_x_assum(qspec_then`Destroyed x`mp_tac) >>
+     simp[fix_inspected_def] ) >>
+  `LENGTH veterans = LENGTH actions` by (
+    unabbrev_all_tac >> simp[localActions_def] )
+  >- (
+    simp[GSYM ZIP_APPEND,MAP_MAP_o] >>
+    simp[MAP_ZIP,LENGTH_REPLICATE] >>
+    simp[REPLICATE_GENLIST,MAP_GENLIST,fix_inspected_def] >>
+    simp[GSYM ZIP_APPEND]
+    simp[set_policies_thm] >>
+    simp[fix_inspected_def] >>
+    ZIP_APPEND
+    ZIP_GENLIST
+    simp[ZIP_MAP]
+    simp[APPEND_LENGTH_EQ,LENGTH_ZIP,MAP_ZIP]
+    match_mp_tac APPEND_EQ
+    f"append_eq"
+    m``l1:'a list ++ l2 = l3 ++ l4``
+
 
 val steph_fill_step = Q.store_thm("steph_fill_step",
   `wf_state_with_hole s ∧
